newest version of flush and fence
now supporting extra resource exchanges

src/high/weakestpre_exp.v
@@ -1,520 +1,538 @@
-From stdpp Require Import gmap.
-From iris.program_logic Require weakestpre.
-
-From stdpp Require Import countable numbers gmap.
-From iris Require Import invariants.
-From iris.proofmode Require Import tactics monpred.
-From iris.algebra Require Import gmap gset excl auth.
-From iris.program_logic Require weakestpre.
-From iris.heap_lang Require Import locations.
+From iris.proofmode Require Import proofmode monpred.
 From iris_named_props Require Import named_props.
-
-From self.algebra Require Export ghost_map.
 From self Require Export extra ipm_tactics solve_view_le.
-From self.high Require Export dprop dprop_liftings.
-From self Require Export view.
-From self Require Export lang.
-From self.base Require Import primitive_laws.
+
+From self.high Require Export dprop.
+From self.base Require Import generational_resources primitive_laws.
+From self.high Require Import
+  generational_resources wrappers crash_weakestpre monpred_simpl modalities protocol locations weakestpre.
+From self.high.lib Require Import abstract_state.
+
 From self.lang Require Import syntax tactics lemmas.
-From self.high Require Import resources crash_weakestpre lifted_modalities
-     monpred_simpl modalities protocol locations.
+From self Require Export lang.
 
-From self.high Require Import weakestpre.
+Section post_fence_sync.
+  Context `{!nvmBaseGS Σ Ω, !nvmHighGS Σ Ω, !PerennialG Σ}.
+  Implicit Types (ℓ : loc).
+  (* For every location we [flush], we will keep the follow tuple,
+   * - [ℓ], the location
+   * - [σ], the abstract state we flush,
+   * - [σ_xchg], the "exchange" state we want to extract resources from,
+   * - [seen ℓ σ_xchg], so that we have the necessary view,
+   * and we also keep enough resource to make three consecutive exchanges/updates with
+   * the protocol in the future and obtain final post condition [R] (when we [flush_sync]),
+   * - [<obj> p_read σ v -∗ □ <obj> P], for getting some basic facts about the physical value,
+   * - [P -∗ <obj> (p_pers σ_old v_old ==∗ <obj> Q ∗ p_pers σ v)] roughly, for the persistent state update,
+   * - [Q -∗ <obj> (p_read σ_xchg v_xchg ==∗ R ∗ p_read σ_xchg v_xchg)] for the read only exchange. *)
+  
+  Definition exchange_3 `{AbstractState ST} ℓ (σ_xchg: ST) (prot: LocationProtocol ST) Q: dProp Σ :=
+    ∀ v_xchg, <obj> (prot.(p_read) σ_xchg v_xchg ==∗ Q ∗ prot.(p_read) σ_xchg v_xchg).
 
-Section wp_rules.
-  Context `{AbstractState ST}.
-  Context `{!nvmG Σ}.
+  (* TODO: include the other case as well *)
+  Definition exchange_2 `{AbstractState ST} ℓ (σ_xchg σ: ST) v (prot: LocationProtocol ST) Q: dProp Σ :=
+    ∀ σ_old v_old,
+    <obj> ((⌜ σ_old ⊑ σ ⌝ -∗ prot.(p_pers) σ_old v_old ==∗
+           prot.(p_pers) σ v ∗ exchange_3 ℓ σ_xchg prot Q) ∧
+           (⌜ σ ⊑ σ_old ⌝ -∗ prot.(p_pers) σ_old v_old ==∗
+           prot.(p_pers) σ_old v_old ∗ exchange_3 ℓ σ_xchg prot Q)).
 
-  Implicit Types (ℓ : loc) (s : ST) (ϕ : ST → val → nvmDeltaG → dProp Σ) (prot: LocationProtocol ST).
-  (* let's try a single location modality, just to make it easier on first attempt *)
+  Definition exchange_1 `{AbstractState ST} ℓ (σ_xchg σ: ST) (prot: LocationProtocol ST) Q: dProp Σ :=
+    ∀ v,
+    <obj> (prot.(p_read) σ v -∗ prot.(p_read) σ v ∗ exchange_2 ℓ σ_xchg σ v prot Q).
 
-  Definition R_progress ℓ prot s Q: dProp Σ :=
-    ∀ s_p v_p v,
-    (* extract the peristent & objective observation *)
-    ∃ P, (prot.(p_read) s v -∗ □ <obj> P) ∗
-         (P -∗
-          (⌜ s_p ⊑ s ⌝ -∗ prot.(p_pers) s_p v_p ==∗ prot.(p_pers) s v ∗ Q) ∧
-          (⌜ s ⊑ s_p ⌝ -∗ prot.(p_pers) s_p v_p ==∗ prot.(p_pers) s_p v_p ∗ Q)).
+  Record FlushInfo := MkFlushInfo {
+    fi_ℓ: loc;
+    fi_ST: Type;
+    fi_ST_eqdec :> EqDecision fi_ST;
+    fi_ST_countable :> Countable fi_ST;
+    fi_ST_is_abstract :> AbstractState fi_ST;
+    fi_prot: LocationProtocol fi_ST;
+    fi_prot_conds :> ProtocolConditions fi_prot;
+    fi_σ: fi_ST;
+    fi_σ_xchg: fi_ST;
+    fi_post: dProp Σ
+  }.
 
-  Definition post_fence_sync_l i ℓ prot (P : dProp Σ): iProp Σ :=
-    let nD := i.2 in
-    ∃ Q, ⌜ Objective Q ⌝ ∗
-      (∃ offset t s, ⌜ {[ ℓ := MaxNat (t - offset) ]} ≼ buffer_view i.1 ⌝ ∗
-                     offset_loc ℓ offset ∗
-                     is_at_loc ℓ ∗
-                     know_protocol ℓ prot ∗
-                     ⎡ know_frag_history_loc ℓ t s ⎤ ∗
-                     R_progress ℓ prot s Q) (∅, ∅, ∅, i.2) ∗
-      (persisted (buffer_view i.1) -∗ (* comes from [fence_sync] instruction *)
-       Q (∅, ∅, ∅, i.2) -∗ (* comes from atomic resrouce exchange at [fence_sync] *)
-       P ((store_view i.1, (flush_view i.1 ⊔ buffer_view i.1), buffer_view i.1), i.2)).
+  #[local] Definition internal_flush_lb `{AbstractState ST} ℓ (prot: LocationProtocol ST) (s : ST) : dProp Σ :=
+    ∃ (t : nat) offset,
+      "#lbBase" ∷ lb_base ℓ prot offset t s ∗
+      (* this assertion is only ever to be used internally, we can safely assert over
+       *  about buffer views. *)
+      "%haveBV" ∷ have_thread_view (∅, ∅, {[ ℓ := MaxNat (t - offset) ]}).
 
-  Program Definition post_fence_sync
-    (ℓ: loc) prot (P : dProp Σ) : dProp Σ :=
-    MonPred (λ i, post_fence_sync_l i ℓ prot P) _.
+  Program Definition post_fence_sync'
+    (P : dProp Σ) : dProp Σ :=
+    MonPred (λ TV,
+      ∃ (fi_list: list FlushInfo),
+        ([∗ list] fi ∈ fi_list,
+           ⎡ is_at_loc fi.(fi_ℓ) ⎤ ∗
+           know_protocol fi.(fi_ℓ) fi.(fi_prot) ∗
+           (* this can probably be promoted to [flush_lb], but doens't seem necessary? *)
+           internal_flush_lb fi.(fi_ℓ) fi.(fi_prot) fi.(fi_σ) ∗
+           seen_state fi.(fi_ℓ) fi.(fi_prot) fi.(fi_σ_xchg) ∗
+           exchange_1 fi.(fi_ℓ) fi.(fi_σ_xchg) fi.(fi_σ) fi.(fi_prot) fi.(fi_post))
+          TV ∗
+        ((persisted (buffer_view TV)) -∗
+         (([∗ list] fi ∈ fi_list, fi.(fi_post)) -∗ P)
+           (store_view TV, (flush_view TV ⊔ buffer_view TV), buffer_view TV))
+      )%I _.
   Next Obligation.
-    intros ???.
-    do 2 intros [[[??]?]?].
-    intros [[[??]?] [= ->]].
-    simpl.
+    intros P. intros [[??]?] [[??]?] [[??]?]. simpl.
     assert (g0 ⊔ g1 ⊑ g3 ⊔ g4). { solve_proper. }
-    rewrite /post_fence_sync_l //=.
-    iIntros "(%Q & % & progress & impl)".
-    iExists Q.
-    iSplit; first done.
-    iSplitL "progress".
-    { iDestruct "progress" as (offset t s) "(%Hincluded & ?)".
-      iExists offset, t, s.
-      iFrame. iPureIntro.
-      etrans; done. }
-    iIntros "persisted Q".
-    iApply monPred_mono; last iApply ("impl" with "[persisted]").
-    { repeat split; done. }
-    { iApply (persisted_anti_mono with "persisted"). done. }
-    { done. }
+    iIntros "(%fi_list & Hfi & P)".
+    iExists fi_list.
+    iSplitL "Hfi".
+    - iApply monPred_mono; last done.
+      solve_view_le.
+    - iIntros "pers".
+      iPoseProof (persisted_anti_mono with "pers") as "pers";
+        (* use the special reasoning to figure out the view automatically. *)
+        last iSpecialize ("P" with "pers"); first done.
+      iApply monPred_mono; last done.
+      solve_view_le.
   Qed.
+End post_fence_sync.
 
-  Lemma wp_flush_lb ℓ prot s st E Q `{!Objective Q}:
-    {{{ store_lb ℓ prot s ∗
-        is_at_loc ℓ ∗
-        <obj> R_progress ℓ prot s Q }}}
+Section weakestpre.
+  Context `{!nvmBaseGS Σ Ω, !nvmHighGS Σ Ω, !PerennialG Σ, AbstractState ST}.
+  
+  Implicit Types (ℓ : loc) (prot: LocationProtocol ST) (σ σ_e: ST) (P Q: dProp Σ).
+  Lemma wp_flush' ℓ prot `{!ProtocolConditions prot} σ_xchg σ st E Q:
+    {{{ ⎡ is_at_loc ℓ ⎤ ∗
+        store_lb ℓ prot σ ∗
+        seen_state ℓ prot σ_xchg ∗
+        exchange_1 ℓ σ_xchg σ prot Q }}}
       Flush #ℓ @ st; E
     {{{ RET #();
-      post_fence_sync ℓ prot (persist_lb ℓ prot s ∗ Q)
+      post_fence_sync' (persist_lb ℓ prot σ ∗ Q)
     }}}.
   Proof.
     intros Φ.
     iModel.
-    destruct TV as [[? ?] ?].
-    iIntros "(#lb & #is_at_loc & progress)".
-    iDestruct "lb" as (tS offset) "H". iNamed "H". iNamed "lbBase".
+    iIntros "(#isAtLoc & #storeLb & #seen & exchange)".
+    iNamed "seen". rename a into t_xchg. rename a0 into offset. rename a1 into msg_xchg. 
+    iDestruct "lbBase" as "(_ & fragHistXchg & #offsetXchg & %tSLeXchg)".
+    iNamed "storeLb". rename a into t. rename a0 into offset'.
+    iNamed "lbBase".
     iDestruct "tSLe" as %tSLe.
-
-    iIntros ([[[??]?] ?] [? [= <-]]) "HΦ".
+    (* remove duplicate offset *)
+    iDestruct (offset_loc_agree with "offset offsetXchg") as %->. iClear "offsetXchg".
+    iIntros (TV' incl) "HΦ".
     iApply wp_unfold_at.
-    iIntros ([[SV PV] BV] incl) "#val".
+    iIntros ([[SV'' PV''] BV''] incl') "#val".
 
     iApply wp_extra_state_interp. { done. } { by apply prim_step_flush_no_fork. }
     (* We open [interp]. *)
     iNamed 1.
 
-    (* Get the points-to predicate. *)
-    iDestruct (know_protocol_extract with "locationProtocol")
-      as "(_ & _ & _ & order & _)".
-    (* TODO: this is weird *)
-    rewrite /know_preorder_loc_d lift_d_at.
-    iDestruct (ghost_map_lookup with "allOrders order") as %look.
-    iDestruct (big_sepM2_dom with "ordered") as %domEq.
-    iDestruct (big_sepM2_dom with "predsFullHold") as %domEq2.
-    assert (is_Some (phys_hists !! ℓ)) as [physHist ?].
-    { apply elem_of_dom. rewrite domEq2 domEq. apply elem_of_dom. naive_solver. }
-    rewrite /offset_loc /is_at_loc /know_frag_history_loc_d 3!lift_d_at.
-    iDestruct (ghost_map_lookup with "offsets offset") as %?.
+    (* offset lookup *)
+    iDestruct (offset_loc_crashed_at_agree with "[$] [$]") as %offsetLook.
+    
+    (* lookup [msg_xchg] early for for [wp_flush] *)
+    iAssert ⌜ ∃ pHist, phys_hists !! ℓ = Some pHist ∧ pHist !! t_xchg = Some msg_xchg ⌝%I as %[pHist [HphysHistLook HpHistLookXchg]].
+    { iPoseProof (auth_map_map_auth_frag with "[$] [$knowPhysMsg]") as "$". }
+    
+    (* obtain mapsto assertion from [interp] to apply base Spirea [wp_flush]. *)
     iDestruct (big_sepM_lookup_acc with "ptsMap") as "[pts ptsMap]".
-    { apply map_lookup_zip_with_Some. naive_solver. }
+    { naive_solver. }
 
-    iApply (wp_flush (extra := {| extra_state_interp := True |}) with "pts").
+    iApply (wp_flush_alt (extra := {| extra_state_interp := True |}) with "pts").
     iNext. iIntros "pts".
-    iDestruct ("ptsMap" with "pts") as "ptsMap".
+    iSpecialize ("ptsMap" with "pts").
 
-    assert (tS - offset ≤ SV !!0 ℓ) as tSLe2.
+    (* view related pure facts. *)
+    assert (t - offset ≤ SV'' !!0 ℓ) as tSLe2.
     { etrans; first apply tSLe. simpl.
-      f_equiv. etrans; first apply H1. apply incl. }
+      f_equiv. solve_view_le. }
+    assert (t_xchg - offset ≤ SV'' !!0 ℓ) as tSLeXchg2.
+    { etrans; first apply tSLeXchg. simpl.
+      f_equiv. solve_view_le. }
     rewrite -assoc.
     iSplitPure.
     { repeat split; try done. apply view_le_lub_r. done. }
     iFrame "val".
-    iSplitL "HΦ progress".
-    { iEval (monPred_simpl) in "HΦ". iApply "HΦ".
-      { iPureIntro. split; last done. solve_view_le. }
-      rewrite /post_fence_sync /post_fence_sync_l.
-      iSimpl.
-      iExists Q.
-      iSplit; first done.
-      iSplitL "progress".
-      { iExists offset, tS, s.
-        iSplitPure.
-        { etrans; last apply view_le_l.
-          apply (singleton_mono ℓ (MaxNat (tS - offset)) (MaxNat (SV !!0 ℓ))).
-          rewrite max_nat_included //. }
-        iEval (rewrite /offset_loc lift_d_at).
-        iSplitR; first iApply "offset".
-        iSplitR; first (rewrite /is_at_loc; simpl; iApply "is_at_loc").
-        iSplitR.
-        { rewrite /know_full_pred_d ?lift_d_at.
-          iNamed "locationProtocol".
-          iFrame "#".
-        }
-        iSplitR; first iApply "knowFragHist".
-        rewrite monPred_at_objectively. iApply "progress". }
-      iIntros "#pers Q".
-      rewrite /persist_lb.
-      repeat (rewrite bi.sep_exist_r; iExists _).
-      simpl. rewrite !monPred_at_embed.
-      iFrame "locationProtocol".
-      iFrame "knowFragHist".
-      iFrame "offset".
-      rewrite -?bi.sep_assoc.
-      iSplitPure; first done.
-      simpl.
-      iSplitR.
-      { simpl. iPureIntro.
-        rewrite !lookup_zero_lub.
-        rewrite lookup_zero_singleton.
-        lia. }
-      iSplitR.
-      2: {
-        iApply monPred_mono; last iApply "Q".
-        solve_view_le.
-        repeat first [ apply view_empty_least | split ].
-      }
-      destruct (BV !! ℓ) as [[?]|] eqn:bvLook.
-      * iApply (persisted_persisted_loc_weak with "pers").
-        { apply lookup_join; last done.
-          rewrite lookup_singleton. done. }
-        lia.
-      * iApply (persisted_persisted_loc_weak with "pers").
-        { rewrite lookup_op.
-          rewrite bvLook.
-          rewrite right_id.
-          rewrite lookup_singleton. done. }
-        lia. }
-    iExistsN.
-    iFrame "#∗%".
-  Qed.
 
-  Lemma wp_fence_sync (ℓ: loc) (prot: LocationProtocol ST) `{!ProtocolConditions prot} (st : stuckness) (E : coPset) (P : dProp Σ) :
-    {{{ post_fence_sync ℓ prot P }}} FenceSync @ st; E {{{ RET #(); P }}}.
+    iSplitL "HΦ exchange".
+    { iEval (monPred_simpl) in "HΦ". iApply "HΦ".
+      { iPureIntro. solve_view_le. }
+      iSimpl.
+      iExists ([MkFlushInfo ℓ _ _ _ _ prot _ σ σ_xchg Q]).
+      iSimpl.
+      iSplitR "".
+      - rewrite right_id.
+        iSplitR; first done. (* [is_at_loc] *)
+        iSplitR; first done. (* [know_protocol] *)
+        iSplitR. (* [internal_flush_lb] *)
+        { iExists t, offset. iFrameNamed.
+          iSplitPure; first done.
+          iPureIntro.
+          split; first (split; solve_view_le).
+          apply view_le_lub_l.
+          apply view_le_singleton.
+          eexists.
+          rewrite lookup_singleton.
+          split; first done.
+          lia. }
+        iSplitR. (* [seen_state] *)
+        { iExists t_xchg, offset, msg_xchg. iFrameNamed. iFrame "#".
+          iSplitPure; first done.
+          iApply monPred_mono; last done.
+          pose proof (view_le_r PV'' {[ ℓ := MaxNat (SV'' !!0 ℓ) ]}).
+          solve_view_le.
+          (split; first split); solve_view_le. }
+        rewrite /exchange_1.
+        iIntros (v). iSpecialize ("exchange" $! v).
+        iPoseProof (objective_at with "exchange") as "exchange".
+        iApply "exchange".
+      - iIntros "persisted".
+        rewrite right_id.
+        iIntros ([[SV''' PV'''] BV'''] [[? ?] ?]) "$".
+        iExists t, offset.
+        iFrameNamed.
+        iSplitPure.
+        { etrans; first apply tSLe2. simpl.
+          f_equiv. solve_view_le. }
+        iSplitPure.
+        (* TODO: improve this proof? *)
+        { etrans; first apply tSLe2. simpl.
+          assert ({[ℓ := MaxNat (SV'' !!0 ℓ)]} ⊑ PV''') as Hflush by solve_view_le.
+          apply view_le_singleton in Hflush as [? [Hlook ?]].
+          rewrite /lookup_zero Hlook //. }
+        rewrite /persisted_loc.
+        destruct (BV'' !! ℓ) as [[?]|] eqn:bvLook.
+        * iApply (persisted_persisted_loc_weak with "persisted").
+          { apply lookup_join; last done.
+            rewrite lookup_singleton. done. }
+          lia.
+        * iApply (persisted_persisted_loc_weak with "persisted").
+          { rewrite lookup_op.
+            rewrite bvLook.
+            rewrite right_id.
+            rewrite lookup_singleton. done. }
+          lia. }
+    (* restore [interp] *)
+    iExistsN.
+    iFrameNamed.
+  Qed.
+End weakestpre.
+
+Section weakestpre.
+  Context `{!nvmBaseGS Σ Ω, !nvmHighGS Σ Ω, !PerennialG Σ}.
+
+  (* View summary:
+   * [SV PV BV]: the thead view before [fence_sync] *)
+  Lemma wp_fence_sync' (st : stuckness) (E : coPset) (P : dProp Σ) :
+    {{{ post_fence_sync' P }}} FenceSync @ st; E {{{ RET #(); P }}}.
   Proof.
     intros Φ.
-    iModel. destruct TV as [[sv pv] bv].
-    iIntros "H".
-
-    iIntros ([[[??]?] ?] [view_incl [= <-]]) "HΦ".
+    iModel.
+    destruct TV as [[SV PV] BV].
+    iIntros "PFS".
+    iIntros ([[SV' PV'] BV'] [[? ?] ?]) "HΦ".
     iApply wp_unfold_at.
-    iIntros ([[SV PV] BV] view_incl') "#val".
-    iApply wp_extra_state_interp. { done. } { apply prim_step_fence_sync_no_fork. }
+    iIntros ([[SV'' PV''] BV''] [[? ?] ?]) "#val".
+    (* TODO: move to a separate lemma to prove this for wp alone. *)
+    iApply wp_extra_state_interp. { done. } { by apply prim_step_fence_sync_no_fork. }
+    (* We open [interp]. *)
     iNamed 1.
 
-    set (extra := (Build_extraStateInterp _ _)).
-    iApply wp_fupd.
-
-    (* since the agreement on predicate content is under a later modality, we need to *)
-    iPoseProof (own_all_full_preds_pred with "[$] [-]") as (predFull predsFullLook) "#predFullEquiv".
-    { iDestruct "H" as (??) "[(% & % & % & _ & _ & _ & (? & ? & ? & _) & _) _]". rewrite ?lift_d_at //=. }
-    iPoseProof (own_all_read_preds_pred with "[$] [-]") as (predRead predsReadLook) "#predReadEquiv".
-    { iDestruct "H" as (??) "[(% & % & % & _ & _ & _ & (? & ? & ? & _) & _) _]". rewrite ?lift_d_at //=. }
-    iPoseProof (own_all_pers_preds_pred with "[$] [-]") as (predPers predsPersLook) "#predPersEquiv".
-    { iDestruct "H" as (??) "[(% & % & % & _ & _ & _ & (? & ? & ? & _) & _) _]". rewrite ?lift_d_at //=. }
-
+    (* TODO: move to a separate lemma *)
+    iApply (@program_logic.crash_weakestpre.wpc_wp).
+    iApply @wpc_fupd.
+    iApply @program_logic.crash_weakestpre.wp_wpc.
+    iDestruct "PFS" as (fi_list) "[fi_exchange_list Hpost]".
+    
+    iEval (rewrite monPred_at_big_sepL) in "fi_exchange_list".
+    (* Here comes the difficult part: since we have multiple locations, we need to obtain a [∗ list] of
+     * equivalences under later modality. *)
+    iAssert (▷ [∗ list] fi ∈ fi_list,
+               (∃ encp_full encp_read encp_pers : enc_predicateO,
+                  ⌜predicates_full !! fi.(fi_ℓ) = Some encp_full⌝ ∗ (encp_full ≡ encode_predicate fi.(fi_prot).(p_full)) ∗
+                  ⌜predicates_read !! fi.(fi_ℓ) = Some encp_read⌝ ∗ (encp_read ≡ encode_predicate fi.(fi_prot).(p_read)) ∗
+                  ⌜predicates_pers !! fi.(fi_ℓ) = Some encp_pers⌝ ∗ (encp_pers ≡ encode_predicate fi.(fi_prot).(p_pers))))%I
+      as "#predicatesEquiv".
+    { iApply big_sepL_later.
+      iDestruct (big_sepL_impl_with_resource with "[full_predicates read_predicates pers_predicates] fi_exchange_list []") as "[_ $]".
+      { iNamedAccu. }
+      iIntros "!>" (k fi ?). iNamed 1.
+      iIntros "(_ & knowProtocol & _)".
+      iNamed "knowProtocol".
+      iPoseProof (own_all_full_preds_pred with "[$] [$]") as (? ?) "#p_fullEquiv".
+      iPoseProof (own_all_read_preds_pred with "[$] [$]") as (? ?) "#p_readEquiv".
+      iPoseProof (own_all_pers_preds_pred with "[$] [$]") as (? ?) "#p_persEquiv".
+      iFrame.
+      iNext.
+      iExistsN. iFrame "#%". }
+    
     iApply (primitive_laws.wp_fence_sync (extra := {| extra_state_interp := True |}) with "[//]").
     simpl.
-    monPred_simpl.
-    iNext. iIntros "#pers".
-    cbn.
-    iDestruct "H" as (Q?) "[(%offset & %tS & %s & (%HtS & #offset & #atLoc & #knowProtocol & (%encS & %Hencode & knowHistFrag) & progress)) H]".
-    simpl in HtS.
-    rewrite /offset_loc lift_d_at.
-    iPoseProof (ghost_map_lookup with "offsets offset") as "%".
-    iPoseProof (ghost_map_map.full_map_frag_entry with "history knowHistFrag") as (absHist) "[% %absHistLook]".
-    (* gather the physical value for the modal timestamp *)
-    iAssert ⌜ is_Some (phys_hists !! ℓ) ⌝%I as (physHist) "%physHistsLook". {
-      iDestruct (big_sepM2_dom with "predsFullHold") as %domEq.
-      iPureIntro.
-      rewrite -elem_of_dom domEq elem_of_dom.
-      by eexists.
-    }
-    iAssert ⌜ is_Some (physHist !! tS) ⌝%I as (msg) "%physHistLook". {
-      iDestruct (big_sepM2_lookup with "predsFullHold") as "(% & % & ? & ? & Hlook)";
-        [ exact: physHistsLook | done | ].
-      iDestruct (big_sepM2_dom with "Hlook") as %domEq.
-      iPureIntro.
-      rewrite -elem_of_dom domEq elem_of_dom.
-      by eexists.
-    }
-
-    (* We now extract the old [p_pers] assertion *)
-    iDestruct (big_sepM2_delete with "predsPersHold")
-      as "[(%predPers' & %tP & %encSP & %msgP & % & %localPView & % & % & predPersHolds) predsPersRest]";
-      [ exact physHistsLook | done | ].
-    replace (predPers') with (predPers); last by simplify_map_eq.
-    iAssert (⌜ ∃ SP, decode encSP = Some SP ⌝)%I as (SP) "%eqP". {
-      iDestruct "predPersHolds" as (PP) "[#eqP _]".
-      iEval (rewrite discrete_fun_equivI) in "predPersEquiv".
-      iSpecialize ("predPersEquiv" $! encSP).
-      iEval (rewrite discrete_fun_equivI) in "predPersEquiv".
-      iSpecialize ("predPersEquiv" $! (msg_val msgP)).
-      iRewrite "predPersEquiv" in "eqP".
-      iPoseProof (encode_predicate_decode (p_pers prot) encSP (msg_val msgP) PP with "eqP") as (SP) "%decodeSP".
-      iExists _. done.
-    }
-    iPoseProof (predicate_holds_phi_decode with "predPersEquiv predPersHolds") as "pred_pers_holds";
-      first done.
-    (* before anything, we first construct the updated [global_pview] *)
-    set global_pview' := (global_pview ⋅ {[ ℓ := MaxNat (tS - offset) ]}).
-    (* proof that we know [global_pview'] is persisted. *)
-    iAssert (persisted global_pview')%I with "[]" as "#globalPViewPersisted'". {
-      rewrite /global_pview' /persisted.
-      iCombine "globalPViewPersisted pers" as "newGlobalPViewPersisted".
-      iApply (own_mono with "newGlobalPViewPersisted").
-      apply auth_frag_mono, cmra_mono_l.
-      etrans; last apply view_incl'.
-      etrans; last apply view_incl.
-      done.
-    }
-    (* since we are dealing with the persisted view here, might as well simplify the modality resource *)
-    iDestruct ("H" with "[pers]") as "H".
-    { iApply persisted_weak; last iApply "pers". etrans; [ apply view_incl | apply view_incl' ]. }
-
-    set predsFullHold := (([∗map] _ ↦ _; _ ∈ _; _, ∃ _ _, ⌜ predicates_full !! _ = _ ⌝ ∗ _))%I.
-    set predsReadHold := (([∗map] _ ↦ _; _ ∈ _; _, ∃ _ _, ⌜ predicates_read !! _ = _ ⌝ ∗ _))%I.
-    set predReadHolds := (encoded_predicate_holds
-                            predRead
-                            encS
-                            (msg_val msg)
-                            ((default
-                                (msg_store_view msg)
-                                (na_views !! ℓ),
-                                msg_persisted_after_view msg, ∅, gnames)))%I.
-    (* TODO: refactor this part into a separate lemma as I recall several places requires
-     * this proof in one form or another. *)
-    iAssert (predReadHolds ∗ (predReadHolds -∗ predsFullHold ∗ predsReadHold))%I
-      with "[predsReadHold predsFullHold]" as "[predReadHolds predRest]". {
-      iDestruct (big_sepM2_lookup_acc with "predsReadHold") as "[(%predRead' & %offset' & % & % & predReadHolds) predsReadRest]";
-        [ exact: physHistsLook | done | ].
-      assert (offset' = offset) as -> by by simplify_map_eq.
-      assert (predRead' = predRead) as -> by by simplify_map_eq.
-      iDestruct (big_sepM2_lookup_acc with "predsFullHold") as "[(%predFull' & %offset' & % & % & predFullHolds) predsFullRest]";
-        [ exact: physHistsLook | done | ].
-      replace predFull' with predFull; last by simplify_map_eq.
-      replace offset' with offset; last by simplify_map_eq.
-      iPoseProof (big_sepM2_sep with "[$predReadHolds $predFullHolds]") as "predBothHolds".
-      iDestruct (big_sepM2_lookup_acc with "predBothHolds") as "[predBothHolds predBothRest]";
-        [ exact: physHistLook | done | ].
-      destruct (decide (offset ≤ tS ∧ physHist !! S tS = None)) as [[] | Hneg ].
-      - iDestruct "predBothHolds" as "[_ predFullHolds]".
-        iSpecialize ("predFullHolds" with "[//] [//]").
-        iPoseProof (predicate_holds_phi_decode with "predFullEquiv predFullHolds") as "pred_full_holds";
-          first done.
-        iEval (rewrite full_read_split) in "pred_full_holds".
-        iDestruct "pred_full_holds" as "[pred_read_holds p_remaining]".
-        iPoseProof (predicate_holds_phi_decode with "predReadEquiv pred_read_holds") as "PredReadHolds";
-          first done.
-        iFrame.
-        iIntros "predReadHolds".
-        iPoseProof (predicate_holds_phi_decode with "predReadEquiv predReadHolds") as "pred_read_holds";
-          first done.
-        iSpecialize ("p_remaining" with "pred_read_holds").
-        iPoseProof (predicate_holds_phi_decode with "predFullEquiv p_remaining") as "predFullHolds";
-          first done.
-        iSpecialize ("predBothRest" with "[predFullHolds]").
-        { iSplitL ""; first (iIntros ([ | [? ?] ]); [ lia | by simplify_eq ]).
-          iIntros (_ _).
-          iFrame. }
-        iPoseProof (big_sepM2_sep with "predBothRest") as "[predReadHolds predFullHolds]".
-        iSpecialize ("predsReadRest" with "[predReadHolds]").
-        { iExists _, _. by iFrame. }
-        iSpecialize ("predsFullRest" with "[predFullHolds]").
-        { iExists _, _. by iFrame. }
-        iFrame.
-      - iDestruct "predBothHolds" as "[predReadHolds _]".
-        iSpecialize ("predReadHolds" with "[%]").
-        { rewrite not_and_l in Hneg.
-          destruct Hneg as [ | ].
-          - left. lia.
-          - right. rewrite -not_eq_None_Some //=. }
-        iFrame.
-        iIntros "predReadHolds".
-        iSpecialize ("predBothRest" with "[predReadHolds]").
-        { iSplitR ""; first (iIntros (_); iFrame).
-          iIntros (? ?).
-          tauto. }
-        iPoseProof (big_sepM2_sep with "predBothRest") as "[predReadHolds predFullHolds]".
-        iSpecialize ("predsReadRest" with "[predReadHolds]").
-        { iExists _, _. by iFrame. }
-        iSpecialize ("predsFullRest" with "[predFullHolds]").
-        { iExists _, _. by iFrame. }
-        iFrame.
-    }
-    iPoseProof (predicate_holds_phi_decode with "predReadEquiv predReadHolds") as "pred_read_holds";
-      first done.
-    (* we now have enough resrouce to specialize the progress resource *)
-    iDestruct ("progress" $! SP (msg_val msgP) (msg_val msg))
-      as (Pread) "[readExtract progress]".
-    iEval (rewrite ?monPred_at_wand) in "readExtract".
-    iDestruct ("readExtract" with "[%] pred_read_holds") as "#readExtract".
-    { simpl. split; [ solve_view_le | done ]. }
-    iEval (rewrite ?monPred_at_objectively) in "readExtract".
-    iEval (rewrite monPred_at_wand) in "progress".
-    set new_pers_view := (default (msg_store_view msg) (na_views !! ℓ), msg_persisted_after_view msg, ∅, gnames).
-    iSpecialize ("progress" $! new_pers_view with "[%] readExtract").
-    { simpl. split; [ solve_view_le | done ]. }
-    (* now we restore the read predicates *)
-    iPoseProof (predicate_holds_phi_decode with "predReadEquiv pred_read_holds") as "predReadHolds";
-      first done.
-    iDestruct ("predRest" with "[$]") as "[predsFullHold predsReadHold]".
-    (* we need to extract the encoded relation from state interpretation *)
-    iAssert ⌜∃ order, (orders !! ℓ = Some order) ∧ increasing_map order absHist⌝%I
-        as %(order & ordersLook & increasing). {
-      iAssert ⌜is_Some (orders !! ℓ)⌝%I as %[order ordersLook]. {
-        iPoseProof (big_sepM2_dom with "ordered") as "%domEq".
-        rewrite -elem_of_dom -domEq elem_of_dom //.
-      }
-      iPoseProof (big_sepM2_lookup with "ordered") as "%orderLook";
-        [ done | done | by iExists _ ].
-    }
-    iPoseProof (orders_lookup with "[$] []") as "%orderDecode";
-      [ exact ordersLook | | ].
-    { iNamed "knowProtocol". iEval (rewrite lift_d_at) in "knowPreorder". iFrame "#". }
-    subst order.
-    (* to merge proofs after the case analysis *)
-    (* I don't want to do it, but I found no choice... *)
-    iAssert (|==> ([∗map] k↦y1;y2 ∈ phys_hists;abs_hists,
-                   ∃ (pred_pers : positive → val → optionO (dPropO Σ)) (t : nat) (encS0 : positive) (msg0 : message),
-                     ⌜predicates_pers !! k = Some pred_pers⌝ ∗
-                     ⌜view_slice.offsets_add offsets global_pview' !! k = Some t ∨
-                      global_pview' !! k = None ∧ offsets !! k = Some t⌝ ∗
-                     ⌜y2 !! t = Some encS0⌝ ∗ ⌜y1 !! t = Some msg0⌝ ∗
-                     encoded_predicate_holds pred_pers encS0
-                       (msg_val msg0)
-                       (default (msg_store_view msg0) (na_views !! k),
-                        msg_persisted_after_view msg0, ∅, gnames)) ∗ Q new_pers_view)%I
-      with "[predsPersRest pred_pers_holds progress]" as "> [predsPersHold Q]". {
-      (* we are at the point to distinguish whether the flushed state [tS ↦ s, msg] comes later or
-       * the current global persistent timestamp [tP ↦ sP, msgP] comes later.
-       * this is "decidable" since the history is strictly increasing, and comparison between
-       * [tS] and [tP] gives up the answer. *)
-      destruct (decide (tS ≤ tP)).
-      - (* [tS ≤ tP], persistent view unchanged. *)
-        assert (s ⊑ SP). {
-          destruct (decide (tS = tP)) as [ -> | ].
-          - by simplify_map_eq.
-          - specialize (increasing tS tP encS encSP ltac:(lia) ltac:(done) ltac:(done)).
-            by eapply (encode_relation.encode_relation_decode_iff_1) in increasing.
-        }
-        iDestruct "progress" as "[_ progress]".
-        iSpecialize ("progress" with "[//]").
-        iMod ("progress" with "[pred_pers_holds]") as "[pred_pers_holds Q]".
-        { iPoseProof (view_objective_view_objectively with "pred_pers_holds") as "P".
-          iPoseProof (monPred_at_view_objectively with "P") as "P".
-          iApply "P". }
-        iAssert (p_pers prot SP (msg_val msgP)
-                        (default (msg_store_view msgP) (na_views !! ℓ),
-                           msg_persisted_after_view msgP, ∅, gnames))%I with "[pred_pers_holds]" as "pred_pers_holds".
-        { iPoseProof (view_objective_view_objectively with "pred_pers_holds") as "P".
-          iPoseProof (monPred_at_view_objectively with "P") as "P".
-          iApply "P". }
-        iFrame.
-        iPoseProof (predicate_holds_phi_decode with "predPersEquiv pred_pers_holds") as "predPersHolds";
-          first done.
+    iNext. iIntros "#persisted".
+    (* before we apply the exchanges, we need to first combine [p_pers] with [global_pview] assertion.
+     * TODO: make it better? ... *)
+    iAssert (∃ global_pview', ⌜ dom global_pview' ⊆ dom abs_hists ⌝ ∗
+            ([∗ map] ℓ ↦ phys_hist;abs_hist ∈ phys_hists;abs_hists,
+               ∃ encp_pers (t offset: nat) encσ msg,
+                 ⌜ predicates_pers !! ℓ = Some encp_pers ⌝ ∗
+                 ⌜ offsets !! ℓ = Some offset ⌝ ∗
+                 ⌜ abs_hist !! t = Some encσ ⌝ ∗
+                 ⌜ phys_hist !! t = Some msg ⌝ ∗
+                 ⌜ Nat.add offset (global_pview' !!0 ℓ) = t ⌝ ∗
+                 default emp (persisted_loc ℓ <$> (max_nat_car <$> (global_pview' !! ℓ))) ∗
+                 encoded_predicate_holds encp_pers encσ msg.(msg_val) (∅, ∅, ∅)))%I with "[predsPersHold]" as "predsP".
+    { iExists global_pview.
+      iFrame "∗#%". }
+    clear histPViewDoms global_pview.
+    (* Let's deal with the exchanges *)
+    iDestruct (big_sepL_fupd_with_resource _ (λ _ fi, fi.(fi_post) (SV, PV ⊔ BV, BV))%I with
+                "[-fi_exchange_list] fi_exchange_list []") as ">[R Hfi_post]".
+    { iNamedAccu. }
+    { iIntros "!>" (k fi HfiLook). iNamed 1.
+      iIntros "(#isAtLoc & #knowProtocol & #flushLb & #seen & exchange)".
+      iNamed "seen". rename a into t_xchg. rename a0 into offset. rename a1 into msg_xchg.
+      iDestruct "lbBase" as "(_ & fragHistXchg & #offsetXchg & %tSLeXchg)".
+      iNamed "flushLb". rename a into t. rename a0 into offset'.
+      destruct haveBV as [_ haveBV].
+      iNamed "lbBase".
+      iDestruct "tSLe" as %tSLe.
+      (* Extract the precious equality we obtained earlier. *)
+      iDestruct (big_sepL_lookup _ _ k with "predicatesEquiv")
+        as (encp_full encp_read encp_pers) "(% & pFullEquiv & % & pReadEquiv & % & pPersEquiv)"; first done.
+      
+      (* remove duplicate offset *)
+      iDestruct (offset_loc_agree with "offset offsetXchg") as %->. iClear "offsetXchg".
+      (* also obtain offset lookup equality *)
+      iAssert ⌜ offsets !! fi.(fi_ℓ) = Some offset ⌝%I with "[offsets]" as "%".
+      {  iDestruct "offset" as (OCV) "[offsets' %Heq]". 
+        iDestruct (crashed_at_offset_agree with "offsets offsets'") as "%".
+        iPureIntro.
         simplify_map_eq.
-        iPoseProof (big_sepM2_insert_delete with "[predsPersRest predPersHolds]") as "predsPersHold".
-        { iFrame. iExistsN. iFrame. iFrame "%". }
-        do 2 (rewrite insert_id; last done).
-        iModIntro.
-        iApply (big_sepM2_impl with "predsPersHold").
-        iIntros (ℓ' absHist' physHist' ??) "!> (% & % & % & % & ? & %localPView' & ? & ?)".
-        iExists _, _, _, _.
-        iFrame.
-        iPureIntro.
-        destruct (decide (ℓ = ℓ')) as [<- | ].
-        + simpl.
-          destruct localPView as [ localPView | [ pViewLook offsetLook' ] ].
-          * left.
-            rewrite map_lookup_zip_with_Some in localPView.
-            destruct localPView as (offset' & [pview] & ? & ? & eq).
-            simplify_eq.
-            destruct localPView' as [ <- | [] ]; last congruence.
-            rewrite ?map_lookup_zip_with lookup_op lookup_singleton //=.
-            replace (offsets !! ℓ) with (Some offset) by done.
-            rewrite eq //=.
-            f_equal.
-            lia.
-          * simplify_eq.
-            left.
-            rewrite map_lookup_zip_with lookup_op pViewLook lookup_singleton //=.
-            replace (offsets !! ℓ) with (Some offset) by done.
-            simpl.
-            replace (tS - offset) with 0 by lia.
-            rewrite map_lookup_zip_with_Some in localPView'.
-            destruct localPView' as [ (offset' & [pview] & ? & ? & eq) | [] ]; first congruence.
-            simplify_eq.
-            f_equal.
-            lia.
-        + rewrite map_lookup_zip_with lookup_op lookup_singleton_ne ?op_None_right_id //=.
-          rewrite map_lookup_zip_with in localPView'.
-          apply localPView'.
-      - (*we have [tS ≥ tP], which means the new persistent view will be updated. *)
-        specialize (increasing tP tS encSP encS ltac:(lia) ltac:(done) ltac:(done)).
-        eapply (encode_relation.encode_relation_decode_iff_1) in increasing;
-          [ | done | done ].
-        iDestruct "progress" as "[progress _]".
-        iDestruct ("progress" with "[//] [pred_pers_holds]") as "> [new_pred_pers_holds $]".
-        { iPoseProof (view_objective_view_objectively with "pred_pers_holds") as "P".
-          iPoseProof (monPred_at_view_objectively with "P") as "P".
-          iApply "P". }
-        iPoseProof (predicate_holds_phi_decode with "predPersEquiv new_pred_pers_holds") as "predPersHolds";
-          first done.
-        iApply (big_sepM2_delete);
-          [ done | done | ].
-        iSplitL "predPersHolds".
-        { iExistsN. iFrame. iFrame "%".
-          iPureIntro. left.
-          destruct localPView as [ localPView | [ pViewLook offsetLook' ] ].
-          - rewrite map_lookup_zip_with_Some in localPView.
-            destruct localPView as (offset' & [pview] & ? & ? & eq).
-            simplify_eq.
-            rewrite ?map_lookup_zip_with lookup_op lookup_singleton //=.
-            replace (offsets !! ℓ) with (Some offset) by done.
-            rewrite eq //=.
-            f_equal.
-            lia.
-          - simplify_eq.
-            rewrite map_lookup_zip_with lookup_op pViewLook lookup_singleton //=.
-            replace (offsets !! ℓ) with (Some offset) by done.
-            simpl.
-            f_equal.
-            lia. }
-        iApply (big_sepM2_impl with "predsPersRest").
-        iModIntro.
-        iIntros (ℓ' absHist' physHist' ??) "!> (% & % & % & % & ? & %localPView' & ? & ?)".
-        iExistsN.
-        iFrame.
-        iPureIntro.
-        assert (ℓ ≠ ℓ') by (pose proof (lookup_delete phys_hists ℓ); congruence).
-        rewrite map_lookup_zip_with lookup_op lookup_singleton_ne ?op_None_right_id //=.
-        rewrite map_lookup_zip_with in localPView'.
-        apply localPView'.
-    }
+        rewrite lookup_fmap_Some in Heq.
+        destruct Heq as [? [? ?]].
+        by simplify_eq. }
+      (* [ℓ] is atomic location. *)
+      iPoseProof (location_sets_singleton_included with "[$] [$]") as "%isAtLoc".
+      (* lookup [msg_xchg] *)
+      iAssert ⌜ ∃ pHist, phys_hists !! fi.(fi_ℓ) = Some pHist ∧ pHist !! t_xchg = Some msg_xchg ⌝%I
+          as %[pHist [HphysHistLook HpHistLookXchg]].
+      { iPoseProof (auth_map_map_auth_frag with "[$] [$knowPhysMsg]") as "$". }
+      (* lookup [σ_xchg] *)
+      iAssert ⌜ ∃ aHist encσ_xchg, abs_hists !! fi.(fi_ℓ) = Some aHist ∧ aHist !! t_xchg = Some encσ_xchg ∧ decode encσ_xchg = Some fi.(fi_σ_xchg) ⌝%I
+          as %(aHist & encσ_xchg & HabsHistLook & HaHistLookXchg & HdecodeXchg).
+      { iPoseProof (full_map_frag_singleton_agreee with "[$] [$fragHistXchg]") as "$". }
+      (* lookup [σ] *)
+      iAssert ⌜ ∃ aHist encσ, abs_hists !! fi.(fi_ℓ) = Some aHist ∧ aHist !! t = Some encσ ∧ decode encσ = Some fi.(fi_σ) ⌝%I
+          as %(aHist' & encσ & HabsHistLook' & HaHistLook & Hdecode).
+      { iPoseProof (full_map_frag_singleton_agreee with "[$] [$knowFragHist]") as "$". }
+      (* extracts [ℓ] from order *)
+      iDestruct (big_sepM2_dom with "ordered") as "%domOrders".
+      assert (fi.(fi_ℓ) ∈ dom orders) as [enc_order HordersLook]%elem_of_dom.
+      { set_solver. }
+      iDestruct (orders_lookup with "allOrders []") as "%HorderEncode"; first done.
+      { iNamed "knowProtocol". iAssumption. }
+      
+      (* extract [ℓ] from [predsFR] *)
+      iDestruct (big_sepM2_lookup_acc _ _ _ fi.(fi_ℓ) with "predsFullReadHold") as
+        "[(%encp_full' & %encp_read' & %offset' & %predFullLook' & %predReadLook' & %offsetLook' & predFR) predFRRest]".
+      { done. } { done. }
+      (* extract [ℓ] from [predsP] *)
+      iDestruct ("predsP") as (global_pview) "(%histPViewDoms & predsP)".
+      iDestruct (big_sepM2_delete _ _ _ fi.(fi_ℓ) with "predsP") as
+        "[(%encp_pers' & %t_p_old & %offset'' & %encσ_p_old & %msg_p_old & % & % & % & % & %globalPViewLook & persistedOld & predP) predPRest]".
+      { done. } { done. }
+      (* Try to remove the context as much as possible to make my life easier. *)
+      iFrameNamed.
+      simplify_map_eq.
 
+      (* since we are atomic, remove all [na_views] references *)
+      assert (na_views !! fi.(fi_ℓ) = None) as ->.
+      { rewrite -not_elem_of_dom. set_solver. }
+      simpl default.
+      (* there also exists [msg] *)
+      iAssert ⌜ t ∈ dom pHist ⌝%I
+          as %[msg HpHistLook]%elem_of_dom.
+      { iPoseProof (big_sepM2_dom with "predFR") as "->".
+        iPureIntro. apply elem_of_dom. by eexists. }
+      
+      (* first exchange *)
+      iPoseProof (objective_at _ _ (msg_store_view msg, msg_persisted_after_view msg, ∅) with "exchange") as "exchange".
+      iDestruct (big_sepM2_lookup_acc _ _ _ t with "predFR") as "[predFR predFRAcc]".
+      { done. } { done. }
+      set (predFR := if (decide _) then _ else _).
+      iAssert (predFR ∗ (exchange_2 (fi_ℓ fi) (fi_σ_xchg fi) (fi_σ fi) msg.(msg_val) (fi_prot fi) (fi_post fi)) (∅, ∅, ∅))%I
+        with "[predFR exchange]" as "[predFR exchange]".
+      { iEval (monPred_simpl) in "exchange".
+        subst predFR.
+        destruct (decide _).
+        - iPoseProof (predicate_holds_phi_decode_1 with "[$pFullEquiv] [$]") as "pFull"; first done.
+          (* why is typeclass not working? *)
+          iPoseProof (fi.(fi_prot_conds).(full_read_split) with "pFull") as "[pRead pFullAcc]".
+          (* [exchange_2] unfolds here for some reason? *)
+          Opaque exchange_2.
+          iDestruct ("exchange" with "pRead") as "[pRead exchange]".
+          iSpecialize ("pFullAcc" with "pRead").
+          iPoseProof (predicate_holds_phi_decode_2 with "[$pFullEquiv] [$]") as "pFull"; first done.
+          iFrame.
+          Transparent exchange_2.
+          iApply (objective_at with "exchange").
+        - iPoseProof (predicate_holds_phi_decode_1 with "[$pReadEquiv] [$]") as "pRead"; first done.
+          (* [exchange_2] unfolds here for some reason? *)
+          Opaque exchange_2.
+          iDestruct ("exchange" with "pRead") as "[pRead exchange]".
+          iPoseProof (predicate_holds_phi_decode_2 with "[$pReadEquiv] [$]") as "pRead"; first done.
+          iFrame.
+          Transparent exchange_2.
+          iApply (objective_at with "exchange"). }
+
+      iDestruct ("predFRAcc" with "predFR") as "predFR".
+
+      (* second exchange and update [global_pview] *)
+      iEval (rewrite /exchange_2) in "exchange".
+      (* look into [encoded_predicate_holds] to justify decoding of [encσ_p_old] *)
+      iAssert (⌜ ∃ σ_p_old, decode encσ_p_old = Some σ_p_old ⌝)%I as (σ_p_old) "%HdecodePOld".
+      { iDestruct "predP" as (PP) "[#eqP _]".
+        iEval (rewrite discrete_fun_equivI) in "pPersEquiv".
+        iSpecialize ("pPersEquiv" $! encσ_p_old).
+        iEval (rewrite discrete_fun_equivI) in "pPersEquiv".
+        iSpecialize ("pPersEquiv" $! (msg_val msg_p_old)).
+        iRewrite "pPersEquiv" in "eqP".
+        iPoseProof (encode_predicate_decode fi.(fi_prot).(p_pers) encσ_p_old msg_p_old.(msg_val) PP with "eqP") as (σp) "%".
+        iExists _. done. }
+      iDestruct ("exchange" $! σ_p_old msg_p_old.(msg_val)) as "exchange".
+      iEval (monPred_simpl) in "exchange".
+      (* we are not taking any subjective resource anyway, might as well choose the simplest view. *)
+      iDestruct ("exchange" $! (∅, ∅, ∅)) as "exchange".
+      (* attempt to not duplicate third exchange proof *)
+      set t_p_old := (offset + (global_pview !!0 fi_ℓ fi)).
+      iAssert (|==> exchange_3 (fi_ℓ fi) (fi_σ_xchg fi) (fi_prot fi) (fi_post fi) (∅, ∅, ∅) ∗
+                    if decide (t_p_old ≤ t) then
+                      encoded_predicate_holds encp_pers encσ (msg_val msg) (∅, ∅, ∅)
+                    else
+                      encoded_predicate_holds encp_pers encσ_p_old (msg_val msg_p_old) (∅, ∅, ∅))%I
+        with "[predP exchange]" as ">[exchange predP]".
+      { iPoseProof (big_sepM2_lookup with "ordered") as "%Hinc".
+        { done. } { done. }
+        destruct (decide (t_p_old ≤ t)).
+        - iDestruct "exchange" as "[exchange _]".
+          iPoseProof (predicate_holds_phi_decode_1 _ with "[$pPersEquiv] [$]") as "pPers"; first done.
+          Opaque exchange_3.
+          iDestruct ("exchange" with "[] pPers") as ">[pPers exchange]".
+          { destruct (decide (t_p_old = t)) as [ | ]; first by simplify_map_eq.
+            specialize (Hinc t_p_old t _ _ ltac:(lia) ltac:(done) ltac:(done)).
+            eapply encode_relation.encode_relation_decode_iff_1 in Hinc; done. }
+          Transparent exchange_3.
+          iPoseProof (predicate_holds_phi_decode_2 with "[$pPersEquiv] [$]") as "pPers"; first done.
+          iFrame.
+          done.
+        - iDestruct "exchange" as "[_ exchange]".
+          iPoseProof (predicate_holds_phi_decode_1 _ with "[$pPersEquiv] [$]") as "pPers"; first done.
+          Opaque exchange_3.
+          iDestruct ("exchange" with "[] pPers") as ">[pPers exchange]".
+          { specialize (Hinc t t_p_old _ _ ltac:(lia) ltac:(done) ltac:(done)).
+            eapply encode_relation.encode_relation_decode_iff_1 in Hinc; done. }
+          Transparent exchange_3.
+          iPoseProof (predicate_holds_phi_decode_2 with "[$pPersEquiv] [$]") as "pPers"; first done.
+          iFrame.
+          done. }
+      
+      (* final exchange *)
+      iDestruct (big_sepM2_lookup_acc _ _ _ t_xchg with "predFR") as "[predFR predFRAcc]".
+      { done. } { done. }
+      clear predFR.
+      set (predFR := if (decide (_ ∧ _)) then _ else _).
+      iAssert (|==> predFR ∗ fi.(fi_post) (msg_store_view msg_xchg, msg_persisted_after_view msg_xchg, ∅))%I
+        with "[predFR exchange]" as ">[predFR Hfi_post]".
+      { rewrite /exchange_3.
+        iSpecialize ("exchange" $! msg_xchg.(msg_val)).
+        subst predFR.
+        destruct (decide _).
+        - iPoseProof (predicate_holds_phi_decode_1 with "[$pFullEquiv] [$]") as "pFull"; first done.
+          (* why is typeclass not working? *)
+          iPoseProof (fi.(fi_prot_conds).(full_read_split) with "pFull") as "[pRead pFullAcc]".
+          iEval (monPred_simpl) in "exchange".
+          iDestruct ("exchange" with "pRead") as ">[Hfi_post pRead]".
+          iSpecialize ("pFullAcc" with "pRead").
+          iPoseProof (predicate_holds_phi_decode_2 with "[$pFullEquiv] [$]") as "pFull"; first done.
+          by iFrame.
+          
+        - iPoseProof (predicate_holds_phi_decode_1 with "[$pReadEquiv] [$]") as "pRead"; first done.
+          iEval (monPred_simpl) in "exchange".
+          iDestruct ("exchange" with "pRead") as ">[Hfi_post pRead]".
+          iPoseProof (predicate_holds_phi_decode_2 with "[$pReadEquiv] [$]") as "pRead"; first done.
+          by iFrame. }
+      iModIntro.
+      (* deal with postcondition first *)
+      iSplitR "Hfi_post"; last first.
+      { iDestruct "haveMsg" as %[? ?].
+        iApply (monPred_mono with "Hfi_post").
+        solve_view_le. }
+      iDestruct ("predFRAcc" with "predFR") as "predFR".
+      iDestruct ("predFRRest" with "[predFR]") as "$".
+      { iExistsN. iFrame. done. }
+      (* depends on timestamps, we have two different choices for [global_pview] *)
+      destruct (decide (t_p_old ≤ t)).
+      - set global_pview' := (global_pview ⊔ {[ fi.(fi_ℓ) := MaxNat (t - offset) ]}).
+        iExists global_pview'.
+        iSplitR.
+        { subst global_pview'.
+          rewrite dom_op dom_singleton.
+          iPureIntro.
+          set_solver. }
+        iApply (big_sepM2_delete _ _ _ fi.(fi_ℓ) with "[-]").
+        { done. } { done. }
+        iSplitL "predP".
+        + iExistsN.
+          iFrame "∗#%".
+          subst global_pview' t_p_old.
+          rewrite lookup_zero_lub lookup_op lookup_singleton lookup_zero_singleton -Nat.add_max_distr_l.
+          iSplitPure.
+          * replace (offset + (t - offset)) with (t) by lia.
+            apply Nat.max_r.
+            done.
+          * unfold lookup_zero in *.
+            (* why goal is not substituted automatically? *)
+            destruct (global_pview !! fi.(fi_ℓ)) eqn:Heqn; rewrite Heqn; simpl in *.
+            -- rewrite Nat.max_r; last lia.
+               iApply (persisted_weak with "persisted").
+               etrans; first apply haveBV.
+               etrans; eassumption.
+            -- iApply (persisted_weak with "persisted").
+               etrans; first apply haveBV.
+               etrans; eassumption.
+        + iApply (big_sepM2_impl with "predPRest").
+          iIntros "!>" (ℓ' pHist' aHist' Hlook ?) "H".
+          assert (global_pview' !!0 ℓ' = global_pview !!0 ℓ') as ->.
+          { subst global_pview'.
+            rewrite lookup_zero_lub [ {[ _ := _ ]} !!0 _ ]/lookup_zero lookup_singleton_ne; first apply Nat.max_0_r.
+            apply lookup_delete_Some in Hlook as [? ?]. done. }
+          assert (global_pview' !! ℓ' = global_pview !! ℓ') as ->.
+          { subst global_pview'.
+            rewrite lookup_op lookup_singleton_ne; first by rewrite right_id.
+            apply lookup_delete_Some in Hlook as [? ?]. done. }
+          done.
+      - iExists global_pview.
+        iFrame "#%".
+        iApply (big_sepM2_delete _ _ _ fi.(fi_ℓ) with "[predP persistedOld $predPRest]").
+        { done. } { done. }
+        iExistsN.
+        iFrame "∗#%".
+        done. }
     iModIntro.
-    iEval (rewrite -?bi.sep_assoc -and_assoc).
-    iSplit; first solve_view_le.
-    iSplit; first done.
-    iSplitL "HΦ H Q". {
-      iApply "HΦ".
-      - iPureIntro.
-        rewrite -?and_assoc.
-        solve_view_le.
-      - iEval (simpl) in "H".
-        iApply (monPred_mono); last iApply "H".
-        { repeat (first [ apply join_mono | by solve_view_le | split ]). }
-        iApply (objective_at with "Q").
-    }
+    iNamed "R".
+    iSpecialize ("Hpost" with "[] [Hfi_post]").
+    { iApply (persisted_weak with "[$]"). by etrans. }
+    { by iApply monPred_at_big_sepL. }
+    iEval (rewrite monPred_at_wand) in "HΦ".
+    iDestruct ("HΦ" with "[] [Hpost]") as "$".
+    { iPureIntro. solve_view_le. }
+    { iApply monPred_mono; last done.
+      split; last solve_view_le.
+      split; first solve_view_le.
+      f_equiv; solve_view_le. }
+    iFrame "val".
+    iSplitPure; first solve_view_le.
     rewrite /interp.
+    iDestruct "predsP" as (global_pview') "[%histPViewDoms predsPersHold]".
     iExistsN.
-    iClear "globalPViewPersisted".
-    iFrame "ptsMap offsets physHist oldViewsDiscarded crashedAt history historyFragments".
-    iFrame "full_predicates read_predicates pers_predicates".
-    iFrame "allOrders globalPViewPersisted' naLocs atLocs naView atLocsHistories".
-    iFrame "ordered predsFullHold predsReadHold predsPersHold allBumpers bumpMono bumperSome".
-    repeat (iSplitPure; first done).
-    iSplitPure.
-    { rewrite dom_op.
-      apply union_least; first done.
-      rewrite dom_singleton_L singleton_subseteq_l elem_of_dom //. }
-    repeat (iSplitPure; first done).
-    repeat (iSplit; first iAssumption).
-    done.
+    iFrameNamed.
   Qed.
-End wp_rules.
+End weakestpre.
